formalization/Dinic_Maxflow/Preflow_Push_Impl.thy
@@ -1,14 +1,173 @@
 theory Preflow_Push_Impl
 imports 
-  (*"../../../../isafol/DRAT/Array_Map_Default"*)
+  "../../../../isafol/DRAT/Synth_Definition"
+  "../../../../isafol/DRAT/DRAT_Misc"
   Preflow Graph_Impl
   "$AFP/Refine_Imperative_HOL/IICF/IICF"
 begin
 
+(* TODO: Move *)  
+  
+thm WHILEIT_rule  
+  
+lemma monadic_WHILEIT_refine[refine]:  
+  assumes [refine]: "(s',s) \<in> R"
+  assumes [refine]: "\<And>s' s. \<lbrakk> (s',s)\<in>R; I s \<rbrakk> \<Longrightarrow> I' s'"  
+  assumes [refine]: "\<And>s' s. \<lbrakk> (s',s)\<in>R; I s; I' s' \<rbrakk> \<Longrightarrow> b' s' \<le>\<Down>bool_rel (b s)"
+  assumes [refine]: "\<And>s' s. \<lbrakk> (s',s)\<in>R; I s; I' s'; nofail (b s); inres (b s) True \<rbrakk> \<Longrightarrow> f' s' \<le>\<Down>R (f s)"
+  shows "monadic_WHILEIT I' b' f' s' \<le>\<Down>R (monadic_WHILEIT I b f s)"
+  unfolding monadic_WHILEIT_def
+  by (refine_rcg bind_refine'; assumption?; auto)
+  
+lemma monadic_WHILEIT_refine_WHILEIT[refine]:  
+  assumes [refine]: "(s',s) \<in> R"
+  assumes [refine]: "\<And>s' s. \<lbrakk> (s',s)\<in>R; I s \<rbrakk> \<Longrightarrow> I' s'"  
+  assumes [THEN order_trans,refine_vcg]: "\<And>s' s. \<lbrakk> (s',s)\<in>R; I s; I' s' \<rbrakk> \<Longrightarrow> b' s' \<le> SPEC (\<lambda>r. r = b s)"
+  assumes [refine]: "\<And>s' s. \<lbrakk> (s',s)\<in>R; I s; I' s'; b s \<rbrakk> \<Longrightarrow> f' s' \<le>\<Down>R (f s)"
+  shows "monadic_WHILEIT I' b' f' s' \<le>\<Down>R (WHILEIT I b f s)"
+  unfolding WHILEIT_to_monadic
+  by (refine_vcg; assumption?; auto)
+  
+lemma monadic_WHILEIT_refine_WHILET[refine]:  
+  assumes [refine]: "(s',s) \<in> R"
+  assumes [THEN order_trans,refine_vcg]: "\<And>s' s. \<lbrakk> (s',s)\<in>R \<rbrakk> \<Longrightarrow> b' s' \<le> SPEC (\<lambda>r. r = b s)"
+  assumes [refine]: "\<And>s' s. \<lbrakk> (s',s)\<in>R; b s \<rbrakk> \<Longrightarrow> f' s' \<le>\<Down>R (f s)"
+  shows "monadic_WHILEIT (\<lambda>_. True) b' f' s' \<le>\<Down>R (WHILET b f s)"
+  unfolding WHILET_def
+  by (refine_vcg; assumption?)  
 
+lemma monadic_WHILEIT_pat[def_pat_rules]:
+  "monadic_WHILEIT$I \<equiv> UNPROTECT (monadic_WHILEIT I)"
+  by auto  
+    
+lemma id_monadic_WHILEIT[id_rules]: 
+  "PR_CONST (monadic_WHILEIT I) ::\<^sub>i TYPE(('a \<Rightarrow> bool nres) \<Rightarrow> ('a \<Rightarrow> 'a nres) \<Rightarrow> 'a \<Rightarrow> 'a nres)"
+  by simp
+    
+lemma monadic_WHILEIT_arities[sepref_monadify_arity]:
+  "PR_CONST (monadic_WHILEIT I) \<equiv> \<lambda>\<^sub>2b f s. SP (PR_CONST (monadic_WHILEIT I))$(\<lambda>\<^sub>2s. b$s)$(\<lambda>\<^sub>2s. f$s)$s"
+  by (simp)
+
+lemma monadic_WHILEIT_comb[sepref_monadify_comb]:
+  "PR_CONST (monadic_WHILEIT I)$b$f$s \<equiv> 
+    Refine_Basic.bind$(EVAL$s)$(\<lambda>\<^sub>2s. 
+      SP (PR_CONST (monadic_WHILEIT I))$b$f$s
+    )"
+  by (simp)
+
+  
+(*locale Network_with_Adjm = Network c s t for c :: "'capacity::linordered_idom flow" and s t +
+  fixes am assumes am_is_adj_map: "is_adj_map am"
+begin  
+
+  lemma am_in_rel: "(am,adjacent_nodes) \<in> nat_rel \<rightarrow> \<langle>nat_rel\<rangle>list_set_rel"
+    using am_is_adj_map unfolding is_adj_map_def
+    by (auto simp: adjacent_nodes_def list_set_rel_def in_br_conv)  
+  
+  lemma am_out_V_empty[simp]: "v\<notin>V \<Longrightarrow> am v = []"
+    using am_is_adj_map[unfolded is_adj_map_def, THEN spec, of v] E_ss_VxV by auto
+*)
+  
 context Network 
-begin
+begin  
+  
+(* Custom operations *)  
+  
+(* Residual Graph *)  
+  
+definition cf_get :: "'capacity flow \<Rightarrow> edge \<Rightarrow> 'capacity nres" 
+  where "cf_get cf e \<equiv> do {
+    assert (e\<in>E \<union> E\<inverse>);
+    return (cf e)
+  }"  
+  
+definition cf_set :: "'capacity flow \<Rightarrow> edge \<Rightarrow> 'capacity \<Rightarrow> 'capacity flow nres" 
+  where "cf_set cf e x \<equiv> do {
+    assert (e\<in>E \<union> E\<inverse>);
+    return (cf (e:=x))
+  }"  
+  
+definition cf_init :: "'capacity flow nres" where "cf_init \<equiv> return (op_mtx_new c)"
 
+(* Excess *)  
+definition x_init :: "(node \<Rightarrow> 'capacity) nres" where "x_init \<equiv> return (\<lambda>_. 0)"
+definition x_get :: "(node \<Rightarrow> 'capacity) \<Rightarrow> node \<Rightarrow> 'capacity nres" 
+  where "x_get x u \<equiv> do {
+    assert (u\<in>V);
+    return (x u)
+  }"
+definition x_add :: "(node \<Rightarrow> 'capacity) \<Rightarrow> node \<Rightarrow> 'capacity \<Rightarrow> (node \<Rightarrow> 'capacity) nres"  
+  where "x_add x u \<Delta> \<equiv> do {
+    assert (u\<in>V);
+    return (x(u := x u + \<Delta>))
+  }"
+
+(* Adjacency map *)
+definition am_get :: "(node \<Rightarrow> node list) \<Rightarrow> node \<Rightarrow> node list nres"    
+  where "am_get am u \<equiv> do {
+    assert (u\<in>V);
+    return (am u)
+  }"
+    
+definition am_is_in_V :: "(node \<Rightarrow> node list) \<Rightarrow> node \<Rightarrow> bool nres"
+  where "am_is_in_V am u \<equiv> do {
+    return (am u \<noteq> [])
+  }"
+
+lemma am_is_in_V_correct[THEN order_trans, refine_vcg]: 
+  assumes "(am,adjacent_nodes) \<in> nat_rel \<rightarrow> \<langle>nat_rel\<rangle>list_set_rel"
+  shows "am_is_in_V am u \<le> (spec x. x \<longleftrightarrow> u\<in>V)"
+proof -
+  have "u\<in>V \<longleftrightarrow> adjacent_nodes u \<noteq> {}" unfolding V_def adjacent_nodes_def by auto
+  also have "\<dots> \<longleftrightarrow> am u \<noteq> []" using fun_relD[OF assms IdI[of u]] by (auto simp: list_set_rel_def in_br_conv)
+  finally show ?thesis unfolding am_is_in_V_def by refine_vcg auto
+qed    
+    
+(* Neighbor lists *)
+definition n_init :: "(node \<Rightarrow> node list) \<Rightarrow> (node \<Rightarrow> node list) nres" 
+  where "n_init am \<equiv> return (am( s := [], t := []) )"
+  
+definition n_at_end :: "(node \<Rightarrow> node list) \<Rightarrow> node \<Rightarrow> bool nres" 
+  where "n_at_end n u \<equiv> do {
+    assert (u\<in>V-{s,t});
+    return (n u = [])
+  }"
+    
+definition n_get_hd :: "(node \<Rightarrow> node list) \<Rightarrow> node \<Rightarrow> node nres"    
+  where "n_get_hd n u \<equiv> do {
+    assert (u\<in>V-{s,t} \<and> n u \<noteq> []);
+    return (hd (n u))
+  }"
+
+definition n_move_next :: "(node \<Rightarrow> node list) \<Rightarrow> node \<Rightarrow> (node \<Rightarrow> node list) nres"
+  where "n_move_next n u \<equiv> do {
+    assert (u\<in>V-{s,t} \<and> n u \<noteq> []);
+    return (n (u := tl (n u)))
+  }"
+    
+definition n_reset :: "(node \<Rightarrow> node list) \<Rightarrow> (node \<Rightarrow> node list) \<Rightarrow> node \<Rightarrow> (node \<Rightarrow> node list) nres"
+  where "n_reset am n u \<equiv> do {
+    assert (u\<in>V-{s,t});
+    return (n (u := am u))
+  }"
+    
+(* Labeling *)    
+definition l_init :: "nat \<Rightarrow> (node \<Rightarrow> nat) nres"
+  where "l_init C \<equiv> return ((\<lambda>_. 0)(s := C))"
+    
+definition l_get :: "(node \<Rightarrow> nat) \<Rightarrow> node \<Rightarrow> nat nres"    
+  where "l_get l u \<equiv> do {
+    assert (u \<in> V);
+    return (l u)
+  }"
+
+definition l_set :: "(node \<Rightarrow> nat) \<Rightarrow> node \<Rightarrow> nat \<Rightarrow> (node \<Rightarrow> nat) nres"    
+  where "l_set l u a \<equiv> do {
+    assert (u\<in>V);
+    return (l(u := a))
+  }"
+    
+  
 (* Compute excess explicitly *)  
 
 definition "xf_rel \<equiv> { ((excess f,cf_of f),f) | f. True }"
@@ -47,6 +206,122 @@ lemma cf_of_pp_init_f[simp]: "cf_of pp_init_f = pp_init_cf"
 lemma pp_init_x_rel: "((pp_init_x, pp_init_cf), pp_init_f) \<in> xf_rel"
   unfolding xf_rel_def by auto
   
+(* Algorithms for init and mininum adjacent label computation *)  
+  
+definition "pp_init_xcf2_aux \<equiv> do {
+  let x=(\<lambda>_. 0);
+  let cf=c;
+
+  foreach (adjacent_nodes s) (\<lambda>v (x,cf). do {
+    assert ((s,v)\<in>E);
+    assert (s \<noteq> v);
+    let a = cf (s,v);
+    assert (x v = 0);
+    let x = x( s := x s - a, v := a );
+    let cf = cf( (s,v) := 0, (v,s) := a);
+    return (x,cf)
+  }) (x,cf)
+}"
+
+(* TODO: Move *)  
+lemma adjacent_not_self[simp, intro!]: "v \<notin> adjacent_nodes v"
+  unfolding adjacent_nodes_def using no_self_loop 
+  by auto
+  
+  
+lemma pp_init_xcf2_aux_spec: 
+  shows "pp_init_xcf2_aux \<le> SPEC (\<lambda>(x,cf). x=pp_init_x \<and> cf = pp_init_cf)"
+proof -
+  have ADJ_S_AUX: "adjacent_nodes s = {v . (s,v)\<in>E}"
+    unfolding adjacent_nodes_def using no_incoming_s by auto
+    
+  have CSU_AUX: "c (s,u) = 0" if "u\<notin>adjacent_nodes s" for u
+    using that unfolding adjacent_nodes_def by auto
+      
+  show ?thesis
+    unfolding pp_init_xcf2_aux_def
+    apply (refine_vcg FOREACH_rule[where I="\<lambda>it (x,cf). 
+        x s = (\<Sum>v\<in>adjacent_nodes s - it. - c(s,v)) 
+      \<and> (\<forall>v\<in>adjacent_nodes s. x v = (if v\<in>it then 0 else c (s,v)))
+      \<and> (\<forall>v\<in>-insert s (adjacent_nodes s). x v = 0)
+      \<and> (\<forall>v\<in>adjacent_nodes s. if v\<notin>it then cf (s,v) = 0 \<and> cf (v,s) = c (s,v) else cf (s,v) = c (s,v) \<and> cf (v,s) = c (v,s))
+      \<and> (\<forall>u v. u\<noteq>s \<and> v\<noteq>s \<longrightarrow> cf (u,v) = c (u,v) )
+      \<and> (\<forall>u. u\<notin>adjacent_nodes s \<longrightarrow> cf (u,s) = 0 \<and> cf (s,u) = 0)
+    "])
+    apply (vc_solve simp: it_step_insert_iff simp: CSU_AUX)
+    subgoal for v it by (auto simp: ADJ_S_AUX) 
+    subgoal for u it _ v by (auto split: if_splits)
+    subgoal by (auto simp: ADJ_S_AUX)    
+    subgoal by (auto simp: ADJ_S_AUX)    
+    subgoal by (auto split: if_splits)    
+    (* TODO: This proof is still a bit fragile *)    
+    subgoal for x
+      unfolding pp_init_x_def
+      apply (intro ext)  
+      subgoal for u  
+        apply (clarsimp simp: ADJ_S_AUX outgoing_def; intro conjI)  
+        applyS (auto intro!: sum.reindex_cong[where l=snd] intro: inj_onI)
+        applyS (metis (mono_tags, lifting) Compl_iff Graph.zero_cap_simp insertE mem_Collect_eq)  
+        done
+      done  
+    subgoal for x cf    
+      unfolding pp_init_cf_def
+      apply (intro ext)  
+      apply (clarsimp; auto simp: CSU_AUX)
+      done  
+    done  
+qed      
+    
+definition "pp_init_xcf2 am \<equiv> do {
+  x \<leftarrow> x_init;
+  cf \<leftarrow> cf_init;
+
+  assert (s\<in>V);
+  adj \<leftarrow> am_get am s;
+  nfoldli adj (\<lambda>_. True) (\<lambda>v (x,cf). do {
+    assert ((s,v)\<in>E);
+    assert (s \<noteq> v);
+    a \<leftarrow> cf_get cf (s,v);
+    x \<leftarrow> x_add x s (-a);
+    x \<leftarrow> x_add x v a;
+    cf \<leftarrow> cf_set cf (s,v) 0; 
+    cf \<leftarrow> cf_set cf (v,s) a; 
+    return (x,cf)
+  }) (x,cf)
+}"
+  
+lemma pp_init_xcf2_refine_aux:
+  assumes AM: "(am,adjacent_nodes)\<in>nat_rel\<rightarrow>\<langle>nat_rel\<rangle>list_set_rel"
+  shows "pp_init_xcf2 am \<le> \<Down>Id (pp_init_xcf2_aux)"
+  unfolding pp_init_xcf2_def pp_init_xcf2_aux_def
+  unfolding x_init_def cf_init_def am_get_def cf_get_def cf_set_def x_add_def  
+  apply (simp only: nres_monad_laws)
+  supply LFO_refine[OF fun_relD[OF AM IdI[of s]], refine]
+  apply refine_rcg  
+  using E_ss_VxV  
+  by auto
+  
+  
+lemma pp_init_xcf2_refine[refine2]: 
+  assumes AM: "(am,adjacent_nodes)\<in>nat_rel\<rightarrow>\<langle>nat_rel\<rangle>list_set_rel"
+  shows "pp_init_xcf2 am \<le>\<Down>xf_rel (RETURN pp_init_f)"
+  using pp_init_xcf2_refine_aux[OF AM] pp_init_xcf2_aux_spec pp_init_x_rel
+  by (auto simp: pw_le_iff refine_pw_simps)  
+    
+
+lemma n_init_refine[refine2]: 
+  assumes AM: "(am,adjacent_nodes)\<in>nat_rel\<rightarrow>\<langle>nat_rel\<rangle>list_set_rel"
+  shows "n_init am \<le> (spec c. (c, rtf_init_n) \<in> (nat_rel \<rightarrow> \<langle>nat_rel\<rangle>list_set_rel))"
+proof -
+  have[simp]: "am v = []" if "v\<notin>V" for v
+  proof -
+    from that have "adjacent_nodes v = {}" unfolding adjacent_nodes_def using E_ss_VxV by auto
+    thus ?thesis using fun_relD[OF AM IdI[of v]] by (auto simp: list_set_rel_def in_br_conv)
+  qed
+  show ?thesis      
+    unfolding n_init_def rtf_init_n_def 
+    by (auto simp: pw_le_iff refine_pw_simps list_set_autoref_empty fun_relD[OF AM])
+qed  
     
 definition augment_edge_cf :: "'capacity flow \<Rightarrow> _" where 
   "augment_edge_cf cf \<equiv> \<lambda>(u,v) \<Delta>. (cf)( (u,v) := cf (u,v) - \<Delta>, (v,u) := cf (v,u) + \<Delta>)"
@@ -65,25 +340,25 @@ qed
     
     
     
-definition "push2 x cf \<equiv> \<lambda>(u,v). do {
-  assert ( u\<in>V \<and> v\<in>V );
+definition "push2_aux x cf \<equiv> \<lambda>(u,v). do {
+  assert ( (u,v) \<in> E \<union> E\<inverse> );
+  assert ( u \<noteq> v );
   let \<Delta> = min (x u) (cf (u,v));
   return (x( u := x u - \<Delta>, v := x v + \<Delta> ),augment_edge_cf cf (u,v) \<Delta>)
 }"
     
-lemma push2_refine[refine]: "\<lbrakk>((x,cf),f)\<in>xf_rel; (ei,e)\<in>Id\<times>\<^sub>rId\<rbrakk> \<Longrightarrow> push2 x cf ei \<le> \<Down>xf_rel (push f l e)"
-  unfolding push_def push2_def
+lemma push2_aux_refine: "\<lbrakk>((x,cf),f)\<in>xf_rel; (ei,e)\<in>Id\<times>\<^sub>rId\<rbrakk> \<Longrightarrow> push2_aux x cf ei \<le> \<Down>xf_rel (push f l e)"
+  unfolding push_def push2_aux_def
   apply refine_vcg  
-  apply (vc_solve simp: xf_rel_def)
+  apply (vc_solve simp: xf_rel_def no_self_loop)
   subgoal for u v 
-    unfolding push_precond_def using cfE_of_ss_VxV by auto
-  subgoal for u v 
-    unfolding push_precond_def using cfE_of_ss_VxV by auto
+    unfolding push_precond_def using cfE_of_ss_invE by auto
   subgoal for u v 
     apply (rule conjI)
     subgoal proof -
       assume "Labeling c s t f l"
       then interpret Labeling c s t f l .
+          thm cfE_ss_invE
       assume "push_precond f l (u, v)"    
       then interpret l': push_effect_locale c s t f l u v by unfold_locales
       from l'.excess'_if show ?thesis by (auto simp: l'.\<Delta>_def push_effect_def)
@@ -91,17 +366,149 @@ lemma push2_refine[refine]: "\<lbrakk>((x,cf),f)\<in>xf_rel; (ei,e)\<in>Id\<time
     subgoal unfolding push_effect_def push_precond_def by auto
     done  
   done
+
+definition "push2 x cf \<equiv> \<lambda>(u,v). do {
+  assert ( (u,v) \<in> E \<union> E\<inverse> );
+  xu \<leftarrow> x_get x u;
+  cfuv \<leftarrow> cf_get cf (u,v);
+  cfvu \<leftarrow> cf_get cf (v,u);
+  let \<Delta> = min xu cfuv;
+  x \<leftarrow> x_add x u (-\<Delta>);
+  x \<leftarrow> x_add x v \<Delta>;
+
+  cf \<leftarrow> cf_set cf (u,v) (cfuv - \<Delta>);
+  cf \<leftarrow> cf_set cf (v,u) (cfvu + \<Delta>);
   
-definition "relabel2 cf l u \<equiv> do {
+  return (x,cf)
+}"
+    
+lemma push2_refine[refine]: 
+  assumes "((x,cf),f)\<in>xf_rel" "(ei,e)\<in>Id\<times>\<^sub>rId"
+  shows "push2 x cf ei \<le> \<Down>xf_rel (push f l e)"
+proof -
+  have "push2 x cf ei \<le> \<Down>Id (push2_aux x cf ei)"  
+    unfolding push2_def push2_aux_def
+    unfolding x_get_def x_add_def cf_get_def cf_set_def
+    unfolding augment_edge_cf_def  
+    apply (simp only: nres_monad_laws)  
+    apply refine_rcg  
+    using E_ss_VxV  
+    by auto  
+  also note push2_aux_refine[OF assms]    
+  finally show ?thesis . 
+qed  
+    
+definition (in Network) "min_adj_label_aux cf l u \<equiv> do {
+  assert (u\<in>V);
+  x \<leftarrow> foreach (adjacent_nodes u) (\<lambda>v x. do {
+    assert ((u,v)\<in>E\<union>E\<inverse>);
+    assert (v\<in>V);
+    if (cf (u,v) \<noteq> 0) then 
+      case x of 
+        None \<Rightarrow> return (Some (l v)) 
+      | Some xx \<Rightarrow> return (Some (min (l v) (xx)))
+    else
+      return x
+  }) None;
+
+  assert (x\<noteq>None);
+  return (the x)
+}"
+    
+(* TODO: Move *)  
+lemma (in Network) adjacent_nodes_ss_V: "adjacent_nodes u \<subseteq> V"  
+  unfolding adjacent_nodes_def using E_ss_VxV by auto
+
+lemma (in -) set_filter_xform_aux: 
+  "{ f x | x. ( x = a \<or> x\<in>S \<and> x\<notin>it ) \<and> P x } = (if P a then {f a} else {}) \<union> {f x | x. x\<in>S-it \<and> P x}"    
+  by auto
+    
+lemma (in Labeling) min_adj_label_aux_spec: 
+  assumes PRE: "relabel_precond f l u"
+  shows "min_adj_label_aux cf l u \<le> SPEC (\<lambda>x. x = Min { l v | v. (u,v)\<in>cf.E })"
+proof -
+  have AUX: "cf (u,v) \<noteq> 0 \<longleftrightarrow> (u,v)\<in>cf.E" for v unfolding cf.E_def by auto
+  
+  have EQ: "{ l v | v. (u,v)\<in>cf.E } = { l v | v. v\<in>adjacent_nodes u \<and> cf (u,v)\<noteq>0 }"
+    unfolding AUX
+    using cfE_ss_invE
+    by (auto simp: adjacent_nodes_def)
+  
+  define Min_option :: "nat set \<rightharpoonup> nat" where "Min_option X \<equiv> if X={} then None else Some (Min X)" for X
+      
+  from PRE active_has_cf_outgoing have "cf.outgoing u \<noteq> {}" unfolding relabel_precond_def by auto
+  hence [simp]: "u\<in>V" unfolding cf.outgoing_def using cfE_of_ss_VxV by auto
+  from \<open>cf.outgoing u \<noteq> {}\<close> have AUX2: "\<exists>v. v \<in> adjacent_nodes u \<and> cf (u, v) \<noteq> 0"
+    by (smt AUX Collect_empty_eq Image_singleton_iff UnCI adjacent_nodes_def cf.outgoing_def cf_def converse_iff prod.simps(2))
+      
+  show ?thesis unfolding min_adj_label_aux_def EQ   
+    apply (refine_vcg 
+        FOREACH_rule[where I="\<lambda>it x. x = Min_option { l v | v. v\<in>adjacent_nodes u - it \<and> cf (u,v)\<noteq>0 }"]
+        )  
+    apply (vc_solve simp: Min_option_def it_step_insert_iff set_filter_xform_aux split: if_splits)
+    subgoal unfolding adjacent_nodes_def by auto  
+    subgoal unfolding adjacent_nodes_def by auto  
+    subgoal using adjacent_nodes_ss_V by auto  
+    subgoal using adjacent_nodes_ss_V by auto
+    subgoal by (auto simp: Min.insert_remove)
+    subgoal using AUX2 by auto
+    done    
+qed        
+
+definition "min_adj_label am cf l u \<equiv> do {
+  assert (u\<in>V);
+  adj \<leftarrow> am_get am u;
+  x \<leftarrow> nfoldli adj (\<lambda>_. True) (\<lambda>v x. do {
+    assert ((u,v)\<in> E \<union> E\<inverse>);
+    assert (v\<in>V);
+    cfuv \<leftarrow> cf_get cf (u,v);
+    if (cfuv \<noteq> 0) then do {
+      lv \<leftarrow> l_get l v;
+      case x of 
+        None \<Rightarrow> return (Some lv) 
+      | Some xx \<Rightarrow> return (Some (min lv xx))
+    } else
+      return x
+  }) None;
+
+  assert (x\<noteq>None);
+  return (the x)
+}"
+
+lemma min_adj_label_refine[THEN order_trans, refine_vcg]:
+  assumes "Labeling c s t f l"
+  assumes AM: "(am,adjacent_nodes)\<in>nat_rel\<rightarrow>\<langle>nat_rel\<rangle>list_set_rel"
+  assumes PRE: "relabel_precond f l u"
+  assumes [simp]: "cf = cf_of f"  
+  shows "min_adj_label am cf l u \<le> SPEC (\<lambda>x. x = Min { l v | v. (u,v)\<in>cfE_of f })"  
+proof - 
+  interpret Labeling c s t f l by fact
+
+  have "min_adj_label am (cf_of f) l u \<le> \<Down>Id (min_adj_label_aux (cf_of f) l u)"  
+    unfolding min_adj_label_def min_adj_label_aux_def Let_def
+    unfolding am_get_def cf_get_def l_get_def  
+    apply (simp only: nres_monad_laws)  
+    supply LFO_refine[OF fun_relD[OF AM IdI] _ IdI, refine]
+    apply (refine_rcg)
+    by auto  
+  also note min_adj_label_aux_spec[OF PRE]    
+  finally show ?thesis by simp  
+qed      
+  
+  
+    
+definition "relabel2 am cf l u \<equiv> do {
   assert (u\<in>V - {s,t});
-  let nl = Min { l v | v. v\<in>V \<and> cf (u,v)\<noteq>0 } + 1;
-  return ( l( u := nl) )
+  nl \<leftarrow> min_adj_label am cf l u;
+  l \<leftarrow> l_set l u (nl+1);
+  return l
 }"
 
 lemma relabel2_refine[refine]: 
   assumes "((x,cf),f)\<in>xf_rel"
+  assumes AM: "(am,adjacent_nodes)\<in>nat_rel\<rightarrow>\<langle>nat_rel\<rangle>list_set_rel"
   assumes [simplified,simp]: "(li,l)\<in>Id" "(ui,u)\<in>Id"
-  shows "relabel2 cf li ui \<le> \<Down>Id (relabel f l u)"    
+  shows "relabel2 am cf li ui \<le> \<Down>Id (relabel f l u)"    
 proof -
   have [simp]: "{l v |v. v \<in> V \<and> cf_of f (u, v) \<noteq> 0} = {l v |v. cf_of f (u, v) \<noteq> 0}"
     using cfE_of_ss_VxV[of f] 
@@ -110,62 +517,154 @@ proof -
   show ?thesis
     using assms
     unfolding relabel2_def relabel_def
-    apply refine_vcg  
-    apply (vc_solve simp: xf_rel_def relabel_effect_def Graph.E_def)  
+    unfolding l_set_def  
+    apply (refine_vcg AM)
+    apply (vc_solve simp: xf_rel_def relabel_effect_def)
+    apply auto  
     done
-qed    
+qed
     
-definition "discharge2 x cf l n u \<equiv> do {  
+definition "discharge2 am x cf l n u \<equiv> do {  
   assert (u \<in> V);
-  while\<^sub>T (\<lambda>((x,cf),l,n). x u \<noteq> 0) (\<lambda>((x,cf),l,n). do {
-    v \<leftarrow> selectp v. v\<in>n u;
-    case v of
-      None \<Rightarrow> do {
-        l \<leftarrow> relabel2 cf l u;
-        return ((x,cf),l,n(u := adjacent_nodes u))
-      }
-    | Some v \<Rightarrow> do {
-        assert (v\<in>V);
-        if (cf (u,v) \<noteq> 0 \<and> l u = l v + 1) then do {
+  monadic_WHILEIT (\<lambda>_. True) 
+    (\<lambda>((x,cf),l,n). do { xu \<leftarrow> x_get x u; return (xu \<noteq> 0) } ) 
+    (\<lambda>((x,cf),l,n). do {
+      at_end \<leftarrow> n_at_end n u;
+      if at_end then do {
+        l \<leftarrow> relabel2 am cf l u;
+        n \<leftarrow> n_reset am n u;
+        return ((x,cf),l,n)
+      } else do {
+        v \<leftarrow> n_get_hd n u;
+        cfuv \<leftarrow> cf_get cf (u,v);
+        lu \<leftarrow> l_get l u;
+        lv \<leftarrow> l_get l v;
+        if (cfuv \<noteq> 0 \<and> lu = lv + 1) then do {
           (x,cf) \<leftarrow> push2 x cf (u,v);
           return ((x,cf),l,n)
         } else do {
-          return ((x,cf),l,n( u := n u - {v} ))
+          n \<leftarrow> n_move_next n u;
+          return ((x,cf),l,n)
         }
       }
-  }) ((x,cf),l,n)
+    }) ((x,cf),l,n)
 }"
+
+lemma discharge_structure_refine_aux:
+  assumes SR: "(ni,n)\<in>nat_rel \<rightarrow> \<langle>nat_rel\<rangle>list_set_rel"
+  assumes SU: "(ui,u)\<in>Id"  
+  assumes fNR: "fNi \<le> \<Down>R fN"
+  assumes UIV: "u\<in>V-{s,t}"  
+  assumes fSR: "\<And>v vi vs. \<lbrakk> (vi,v)\<in>Id; v\<in>n u; ni u = v#vs; (v#vs,n u)\<in>\<langle>nat_rel\<rangle>list_set_rel \<rbrakk> 
+    \<Longrightarrow> fSi vi \<le> \<Down>R (fS v)"
+  shows
+  "( do {
+    at_end \<leftarrow> n_at_end ni ui;
+    if at_end then fNi
+    else do {
+      v \<leftarrow> n_get_hd ni ui;
+      fSi v
+    }
+  } ) \<le> \<Down>R (
+
+  do {
+    v \<leftarrow> selectp v. v\<in>n u;
+    case v of
+      None \<Rightarrow> fN
+    | Some v \<Rightarrow> fS v
+  })" (is "?lhs \<le>\<Down>R ?rhs")
+  unfolding n_at_end_def n_get_hd_def
+  apply (simp only: nres_monad_laws)  
+  apply (cases "ni u")
+  subgoal
+    using fun_relD[OF SR SU] SU UIV fNR
+    by (auto simp: list_set_rel_def in_br_conv pw_le_iff refine_pw_simps)
     
+  subgoal for v vs
+    using fun_relD[OF SR SU] SU UIV
+    using fSR[OF IdI[of v], of vs]  
+    apply (clarsimp simp: list_set_rel_def in_br_conv pw_le_iff refine_pw_simps split: option.splits)
+    by fastforce  
+  done    
+  
+lemma xf_rel_RELATES[refine_dref_RELATES]: "RELATES xf_rel" by (auto simp: RELATES_def)
+  
 lemma discharge2_refine[refine]:     
   assumes A: "((x,cf),f) \<in> xf_rel"
-  assumes [simplified,simp]: "(li,l)\<in>Id" "(ni,n)\<in>Id" "(ui,u)\<in>Id"
-  shows "discharge2 x cf li ni ui \<le> \<Down>(xf_rel \<times>\<^sub>r Id \<times>\<^sub>r Id) (discharge f l n u)"  
+  assumes AM: "(am,adjacent_nodes)\<in>nat_rel\<rightarrow>\<langle>nat_rel\<rangle>list_set_rel"
+  assumes [simplified,simp]: "(li,l)\<in>Id" "(ui,u)\<in>Id"
+  assumes NR: "(ni,n)\<in>nat_rel \<rightarrow> \<langle>nat_rel\<rangle>list_set_rel"  
+  shows "discharge2 am x cf li ni ui \<le> \<Down>(xf_rel \<times>\<^sub>r Id \<times>\<^sub>r (nat_rel \<rightarrow> \<langle>nat_rel\<rangle>list_set_rel)) (discharge f l n u)"  
   unfolding discharge2_def discharge_def
-  apply (refine_rcg)
-  apply (vc_solve simp: A)
-  subgoal by (simp add: xf_rel_def)  
-  applyS assumption    
-  subgoal by (auto simp: xf_rel_def Graph.E_def)
-  done  
+  apply (rewrite in "monadic_WHILEIT _ _ \<hole> _" vcg_intro_frame)  
+  apply refine_rcg  
+  apply (vc_solve simp: A NR)
+  subgoal by (simp add: xf_rel_def x_get_def)  
+  subgoal for f l n x cf ni   
+    apply (subst vcg_rem_frame)
+    unfolding n_reset_def cf_get_def l_get_def n_move_next_def  
+    apply (simp only: nres_monad_laws)  
+    apply (rule discharge_structure_refine_aux; (refine_vcg AM)?; (assumption)?)  
+    apply (vc_solve simp: fun_relD fun_relD[OF AM])  
+    subgoal for v vs unfolding xf_rel_def Graph.E_def by auto
+    subgoal for v vs by (auto simp: list_set_rel_def in_br_conv)  
+    done
+  done
     
+(* Algorithm to determine card V and initial queue *)    
     
+lemma V_is_adj_nodes: "V = { v . adjacent_nodes v \<noteq> {} }"
+  unfolding V_def adjacent_nodes_def by auto
     
-definition "relabel_to_front2 \<equiv> do {
-  let xcf = (pp_init_x, pp_init_cf);
-  let l = pp_init_l;
-  let n = rtf_init_n;
+definition "init_CQ N am \<equiv> do {
+  let cardV=0;
+  let Q=[];
+  nfoldli [0..<N] (\<lambda>_. True) (\<lambda>v (cardV,Q). do {
+    assert (v<N);
+    inV \<leftarrow> am_is_in_V am v;
+    if inV then do {
+      let cardV = cardV + 1;
+      if v\<noteq>s \<and> v\<noteq>t then
+        return (cardV,v#Q)
+      else 
+        return (cardV,Q)
+    } else
+      return (cardV,Q)
+  }) (cardV,Q)
+}"    
+
+lemma init_CQ_correct[THEN order_trans, refine_vcg]:
+  assumes V_ss: "V \<subseteq> {0..<N}"
+  assumes AMR: "(am,adjacent_nodes) \<in> nat_rel \<rightarrow> \<langle>nat_rel\<rangle>list_set_rel"  
+  shows "init_CQ N am \<le> SPEC (\<lambda>(C,Q). C = card V \<and> distinct Q \<and> set Q = V-{s,t})"
+  unfolding init_CQ_def  
+  apply (refine_vcg 
+      nfoldli_rule[where I="\<lambda>l1 _ (C,Q). C = card (V\<inter>set l1) \<and> distinct Q \<and> set Q = (V\<inter>set l1)-{s,t} "]
+      AMR
+      )  
+  apply clarsimp_all  
+  using V_ss  
+  apply (auto simp: upt_eq_lel_conv Int_absorb2)  
+  done    
+    
+definition "relabel_to_front2 N am \<equiv> do {
+  (cardV, L_right) \<leftarrow> init_CQ N am;
+
+  xcf \<leftarrow> pp_init_xcf2 am;
+  l \<leftarrow> l_init cardV;
+  n \<leftarrow> n_init am;
 
   let L_left=[];
-  L_right \<leftarrow> spec l. distinct l \<and> set l = V - {s,t};
 
   ((x,cf),l,n,L_left,L_right) \<leftarrow> while\<^sub>T (\<lambda>((x,cf),l,n,L_left,L_right). L_right \<noteq> []) (\<lambda>((x,cf),l,n,L_left,L_right). do {
     assert (L_right \<noteq> []);
     let u = hd L_right;
-    let old_lu = l u;
+    old_lu \<leftarrow> l_get l u;
 
-    ((x,cf),l,n) \<leftarrow> discharge2 x cf l n u;
+    ((x,cf),l,n) \<leftarrow> discharge2 am x cf l n u;
 
-    if (l u \<noteq> old_lu) then do {
+    lu \<leftarrow> l_get l u;
+    if (lu \<noteq> old_lu) then do {
       (* Move u to front of l, and restart scanning L. The cost for rev_append is amortized by going to next node in L *)
       let (L_left,L_right) = ([u],rev_append L_left (tl L_right));
       return ((x,cf),l,n,L_left,L_right)
@@ -177,13 +676,27 @@ definition "relabel_to_front2 \<equiv> do {
 
   }) (xcf,l,n,L_left,L_right);
 
-  return (flow_of_cf cf)
+  return cf
 }"
-
-lemma relabel_to_front2_refine[refine]: "relabel_to_front2 \<le> \<Down>Id relabel_to_front"
+  
+(* TODO: Move to Refine_Basic convenience *)  
+lemma (in -) refine2spec_aux:
+  "a \<le> \<Down>R b \<longleftrightarrow> ( (nofail b \<longrightarrow> a \<le> SPEC ( \<lambda>r. (\<exists>x. inres b x \<and> (r,x)\<in>R) )) )"
+  by (auto simp: pw_le_iff refine_pw_simps)
+  
+lemma (in -) refine2specI:
+  assumes "nofail b \<Longrightarrow> a \<le> SPEC (\<lambda>r. (\<exists>x. inres b x \<and> (r,x)\<in>R) )"
+  shows "a \<le> \<Down>R b"  
+  using assms by (simp add: refine2spec_aux)  
+  
+    
+lemma relabel_to_front2_refine[refine]: 
+  assumes AM: "(am,adjacent_nodes)\<in>nat_rel\<rightarrow>\<langle>nat_rel\<rangle>list_set_rel"
+  assumes V_ss: "V \<subseteq> {0..<N}"
+  shows "relabel_to_front2 N am \<le> \<Down>(br (flow_of_cf) (RPreGraph c s t)) relabel_to_front"
 proof -
   define s_rel :: "(_ \<times> ( 'capacity flow * (nat\<Rightarrow>nat) * (node\<Rightarrow>node set) * node list * node list)) set"
-    where "s_rel \<equiv> xf_rel \<times>\<^sub>r Id \<times>\<^sub>r Id \<times>\<^sub>r br rev (\<lambda>_. True) \<times>\<^sub>r Id"
+    where "s_rel \<equiv> xf_rel \<times>\<^sub>r Id \<times>\<^sub>r (nat_rel \<rightarrow> \<langle>nat_rel\<rangle>list_set_rel) \<times>\<^sub>r br rev (\<lambda>_. True) \<times>\<^sub>r Id"
   
   have [refine_dref_RELATES]: "RELATES s_rel" unfolding RELATES_def ..
       
@@ -191,24 +704,73 @@ proof -
     fix f l n
     assume "neighbor_invar c s t f l n"
     then interpret neighbor_invar c s t f l n .  
-    have "flow_of_cf cf = f" by (rule fo_rg_inv)
+    have G1: "flow_of_cf cf = f" by (rule fo_rg_inv)
+    have G2: "RPreGraph c s t cf" by (rule is_RPreGraph)
+    note G1 G2    
   } note AUX1=this   
       
+  have AUXR: "do {
+      (cardV, L_right) \<leftarrow> init_CQ N am;
+      xcf \<leftarrow> pp_init_xcf2 am;
+      l \<leftarrow> l_init cardV;
+      n \<leftarrow> n_init am;
+      Fi L_right xcf l n
+    }
+    \<le> \<Down>R (do {
+      L_right \<leftarrow> spec l. distinct l \<and> set l = V - {s, t};
+      F L_right
+    })
+  " 
+  if "\<And>L_right xcf n. \<lbrakk> (xcf,pp_init_f)\<in>xf_rel; (n,rtf_init_n) \<in> nat_rel \<rightarrow> \<langle>nat_rel\<rangle>list_set_rel \<rbrakk> 
+    \<Longrightarrow> Fi L_right xcf pp_init_l n \<le> \<Down>R (F L_right)"
+  for Fi F R
+    unfolding l_init_def
+    apply (rule refine2specI)
+    supply pp_init_xcf2_refine[OF AM, unfolded conc_fun_RETURN, THEN order_trans, refine_vcg]  
+    supply n_init_refine[OF AM,THEN order_trans, refine_vcg]  
+    apply (refine_vcg AM V_ss)
+    apply clarsimp  
+    subgoal for L_right x cf n
+      using that[of "(x,cf)" n L_right]
+      unfolding pp_init_l_def  
+      by (clarsimp simp: pw_le_iff refine_pw_simps; meson)  
+    done  
   show ?thesis
-    unfolding relabel_to_front2_def relabel_to_front_def
-    apply refine_rcg  
+    unfolding relabel_to_front2_def relabel_to_front_def Let_def l_get_def
+    apply (simp only: nres_monad_laws)  
+    apply (rule AUXR)  
+    apply (refine_rcg AM)
     apply refine_dref_type
     unfolding s_rel_def
-    apply (vc_solve simp: in_br_conv rev_append_eq pp_init_x_rel xf_rel_def AUX1)
+    apply (vc_solve simp: in_br_conv rev_append_eq xf_rel_def AUX1 fun_relD)
     done  
 qed  
-
+  
 end -- \<open>Network\<close>  
   
-xxx, ctd here:
-  Now we are working directly on residual graph!
-  Insert algorithms for init, and min-computation, then sepref!
-  Should have stuff done for flow_of_cf already!
+  
+definition "fun_rel'\<equiv> fun_rel"
+    
+lemma fun_rel'_id[simp,fcomp_norm_unfold]:
+  "\<langle>Id,Id\<rangle>fun_rel' = Id" unfolding fun_rel'_def by auto 
+  
+  
+context
+  notes [simp] = IS_PRES_EQ_def fun_rel'_def
+begin
+  sepref_decl_op fun_apply: "\<lambda>f x. f x" :: "(\<langle>A,B\<rangle>fun_rel') \<rightarrow> A \<rightarrow> B" .
+  sepref_decl_op fun_update: fun_upd :: "(\<langle>A,B\<rangle>fun_rel') \<rightarrow> A \<rightarrow> B \<rightarrow> \<langle>A,B\<rangle>fun_rel'" where "IS_PRES_EQ A" .
+  sepref_decl_op fun_const: "\<lambda>c _. c" :: "B \<rightarrow> \<langle>A,B\<rangle>fun_rel'" .
+
+  lemma fun_fixed_const_fref: 
+    "\<lbrakk> (ci,c)\<in>B \<rbrakk> \<Longrightarrow> (uncurry0 (return (\<lambda>_. ci)), uncurry0 (return (\<lambda>_. c))) \<in> unit_rel \<rightarrow>\<^sub>f \<langle>\<langle>A,B\<rangle>fun_rel'\<rangle>nres_rel"
+    by (auto intro!: frefI nres_relI)
+      
+end
+
+(* TODO: Move *)  
+  
+lemma uminus_hnr[sepref_import_param]: "(uminus,uminus)\<in>int_rel \<rightarrow> int_rel" by auto  
   
   
 (* TODO: Duplicated from EdmondsKarp_Impl! *)  
@@ -216,14 +778,24 @@ locale Network_Impl = Network c s t for c :: "capacity_impl graph" and s t +
   fixes N :: nat
   assumes V_ss: "V\<subseteq>{0..<N}"
 begin  
+  lemma nwi_this: "Network_Impl c s t N" by unfold_locales
+  
   lemma E_ss: "E \<subseteq> {0..<N}\<times>{0..<N}" using E_ss_VxV V_ss by auto
 
+      
+  (* Simp setup for side-condition discharging *)    
   lemma mtx_nonzero_iff[simp]: "mtx_nonzero c = E" unfolding E_def by (auto simp: mtx_nonzero_def)
 
   lemma mtx_nonzeroN: "mtx_nonzero c \<subseteq> {0..<N}\<times>{0..<N}" using E_ss by simp
 
+  lemma [simp]: "(u,v) \<in> mtx_nonzero c \<Longrightarrow> u<N \<and> v<N" using mtx_nonzeroN by auto   
+      
   lemma [simp]: "v\<in>V \<Longrightarrow> v<N" using V_ss by auto
   
+  lemma [simp]: "e\<in>E \<or> e\<in>E\<inverse> \<Longrightarrow> case e of (u,v) \<Rightarrow> u<N \<and> v<N"    
+    using E_ss by auto
+  lemmas [simp] = nested_case_prod_simp
+      
   text \<open>Declare some variables to Sepref. \<close>
   lemmas [id_rules] = 
     itypeI[Pure.of N "TYPE(nat)"]  
@@ -237,12 +809,41 @@ begin
     IdI[of s]
     IdI[of t]
     (*IdI[of c]*)
-  
-  text \<open>Function from nodes, with default value\<close>
+
+  lemma [sepref_fr_rules]: 
+    "(uncurry0 (return c),uncurry0 (RETURN c))\<in>unit_assn\<^sup>k \<rightarrow>\<^sub>a pure (nat_rel \<times>\<^sub>r nat_rel \<rightarrow> Id)"
+    by (sepref_to_hoare) sep_auto 
     
+  abbreviation cap_assn :: "capacity_impl \<Rightarrow> _" where "cap_assn \<equiv> id_assn"  
+  definition "cf_assn \<equiv> asmtx_assn N cap_assn"  
+  abbreviation "edge_assn \<equiv> nat_assn \<times>\<^sub>a nat_assn"  
+  abbreviation (input) "node_assn \<equiv> nat_assn"  
+    
+  text \<open>Implementing the basic operations\<close>
+  sepref_register cf_get cf_set cf_init 
+  sepref_thm cf_get_impl is "uncurry (PR_CONST cf_get)" :: "cf_assn\<^sup>k *\<^sub>a edge_assn\<^sup>k \<rightarrow>\<^sub>a cap_assn"  
+    unfolding cf_get_def cf_assn_def PR_CONST_def
+    by sepref
+  concrete_definition (in -) cf_get_impl uses Network_Impl.cf_get_impl.refine_raw is "(uncurry ?f,_)\<in>_"
+      
+  sepref_thm cf_set_impl is "uncurry2 (PR_CONST cf_set)" :: "cf_assn\<^sup>d *\<^sub>a edge_assn\<^sup>k *\<^sub>a cap_assn\<^sup>k \<rightarrow>\<^sub>a cf_assn"  
+    unfolding cf_set_def cf_assn_def PR_CONST_def by sepref
+  concrete_definition (in -) cf_set_impl uses Network_Impl.cf_set_impl.refine_raw is "(uncurry2 ?f,_)\<in>_"
+
+  sepref_thm cf_init_impl is "uncurry0 (PR_CONST cf_init)" :: "unit_assn\<^sup>k \<rightarrow>\<^sub>a cf_assn" 
+    unfolding PR_CONST_def cf_assn_def cf_init_def 
+    apply (rewrite amtx_fold_custom_new[of N N])
+    by sepref  
+  concrete_definition (in -) cf_init_impl uses Network_Impl.cf_init_impl.refine_raw is "(uncurry0 ?f,_)\<in>_"
+  lemmas [sepref_fr_rules] = cf_get_impl.refine[OF nwi_this] cf_set_impl.refine[OF nwi_this] cf_init_impl.refine[OF nwi_this]
+      
+  text \<open>Function from nodes, with default value\<close>
   definition "is_nf dflt f a \<equiv> \<exists>\<^sub>Al. a\<mapsto>\<^sub>al * \<up>(length l = N \<and> (\<forall>i<N. l!i = f i) \<and> (\<forall>i\<ge>N. f i = dflt))"
     
   lemma nf_init_rule[sep_heap_rules]: "<emp> Array.new N dflt <is_nf dflt (\<lambda>_. dflt)>"
+    unfolding is_nf_def by sep_auto
+
+  lemma nf_copy_rule[sep_heap_rules]: "<is_nf dflt f a> array_copy a <\<lambda>r. is_nf dflt f a * is_nf dflt f r>"
     unfolding is_nf_def by sep_auto
     
   lemma nf_lookup_rule[sep_heap_rules]: "v<N \<Longrightarrow> <is_nf dflt f a> Array.nth a v <\<lambda>r. is_nf dflt f a *\<up>(r = f v)>"
@@ -250,35 +851,221 @@ begin
     
   lemma nf_update_rule[sep_heap_rules]: "v<N \<Longrightarrow> <is_nf dflt f a> Array.upd v x a <is_nf dflt (f(v:=x))>"  
     unfolding is_nf_def by sep_auto
+
+  definition "am_assn \<equiv> is_nf ([]::nat list)"    
+  sepref_register am_get  
+  lemma [sepref_fr_rules]: "(uncurry Array.nth, uncurry (PR_CONST am_get)) \<in> am_assn\<^sup>k *\<^sub>a node_assn\<^sup>k \<rightarrow>\<^sub>a list_assn id_assn"  
+    unfolding am_assn_def am_get_def list_assn_pure_conv
+    by sepref_to_hoare (sep_auto simp: refine_pw_simps)
+
+      
+  definition (in -) "am_is_in_V_impl am u \<equiv> do {
+    amu \<leftarrow> Array.nth am u;
+    return (\<not>is_Nil amu)
+  }"    
+  sepref_register am_is_in_V    
+  lemma [sepref_fr_rules]: "(uncurry am_is_in_V_impl, uncurry (am_is_in_V)) 
+    \<in> [\<lambda>(_,v). v<N]\<^sub>a am_assn\<^sup>k *\<^sub>a node_assn\<^sup>k \<rightarrow> bool_assn"  
+    unfolding am_assn_def am_is_in_V_def am_is_in_V_impl_def
+    apply sepref_to_hoare 
+    apply (sep_auto simp: refine_pw_simps split: list.split)
+    done
+      
+  definition "n_assn \<equiv> is_nf ([]::nat list)"    
+      
+  definition (in -) "n_init_impl s t am \<equiv> do {
+    n \<leftarrow> array_copy am;
+    n \<leftarrow> Array.upd s [] n;
+    n \<leftarrow> Array.upd t [] n;
+    return n
+  }"      
+      
+  sepref_register n_init  
+  lemma [sepref_fr_rules]: "(n_init_impl s t,PR_CONST n_init) \<in> am_assn\<^sup>k \<rightarrow>\<^sub>a n_assn" 
+    apply sepref_to_hoare
+    unfolding am_assn_def n_assn_def n_init_impl_def n_init_def
+    by (sep_auto)  
+      
+  definition (in -) "n_at_end_impl n u \<equiv> do {
+    nu \<leftarrow> Array.nth n u;
+    return (is_Nil nu)
+  }"
+      
+  sepref_register n_at_end
+  lemma [sepref_fr_rules]: "(uncurry n_at_end_impl, uncurry (PR_CONST n_at_end)) \<in> n_assn\<^sup>k *\<^sub>a node_assn\<^sup>k \<rightarrow>\<^sub>a bool_assn"  
+    apply sepref_to_hoare unfolding n_at_end_impl_def n_at_end_def n_assn_def
+    by (sep_auto simp: refine_pw_simps split: list.split)
     
+  definition (in -) "n_get_hd_impl n u \<equiv> do {
+    nu \<leftarrow> Array.nth n u;
+    return (hd nu)
+  }"      
+  sepref_register n_get_hd
+  lemma [sepref_fr_rules]: "(uncurry n_get_hd_impl, uncurry (PR_CONST n_get_hd)) \<in> n_assn\<^sup>k *\<^sub>a node_assn\<^sup>k \<rightarrow>\<^sub>a node_assn"  
+    apply sepref_to_hoare unfolding n_get_hd_impl_def n_get_hd_def n_assn_def
+    by (sep_auto simp: refine_pw_simps)
+    
+  definition (in -) "n_move_next_impl n u \<equiv> do {
+    nu \<leftarrow> Array.nth n u;
+    n \<leftarrow> Array.upd u (tl nu) n;
+    return n
+  }" 
+  sepref_register n_move_next
+  lemma [sepref_fr_rules]: "(uncurry n_move_next_impl, uncurry (PR_CONST n_move_next)) \<in> n_assn\<^sup>d *\<^sub>a node_assn\<^sup>k \<rightarrow>\<^sub>a n_assn"  
+    apply sepref_to_hoare unfolding n_move_next_impl_def n_move_next_def n_assn_def
+    by (sep_auto simp: refine_pw_simps)
+    
+  definition (in -) "n_reset_impl am n u \<equiv> do {
+    nu \<leftarrow> Array.nth am u;
+    n \<leftarrow> Array.upd u nu n;
+    return n
+  }"
+  sepref_register n_reset
+  lemma [sepref_fr_rules]: "(uncurry2 n_reset_impl, uncurry2 (PR_CONST n_reset)) \<in> am_assn\<^sup>k *\<^sub>a n_assn\<^sup>d *\<^sub>a node_assn\<^sup>k \<rightarrow>\<^sub>a n_assn"  
+    apply sepref_to_hoare unfolding n_reset_impl_def n_reset_def n_assn_def am_assn_def
+    by (sep_auto simp: refine_pw_simps)
+    
+  definition "x_assn \<equiv> is_nf (0::capacity_impl)"    
+    
+  lemma [sepref_fr_rules]: "(uncurry0 (Array.new N 0), uncurry0 x_init) \<in> unit_assn\<^sup>k \<rightarrow>\<^sub>a x_assn"  
+    apply sepref_to_hoare unfolding x_assn_def x_init_def by sep_auto
+      
+  sepref_register x_get    
+  lemma [sepref_fr_rules]: "(uncurry Array.nth, uncurry (PR_CONST x_get)) \<in> x_assn\<^sup>k *\<^sub>a node_assn\<^sup>k \<rightarrow>\<^sub>a cap_assn"
+    apply sepref_to_hoare unfolding x_assn_def x_get_def by (sep_auto simp: refine_pw_simps)
+      
+  definition (in -) "x_add_impl x u \<Delta> \<equiv> do {
+    xu \<leftarrow> Array.nth x u;
+    x \<leftarrow> Array.upd u (xu+\<Delta>) x;
+    return x
+  }"  
+  sepref_register x_add
+  lemma [sepref_fr_rules]: "(uncurry2 x_add_impl, uncurry2 (PR_CONST x_add)) \<in> x_assn\<^sup>d *\<^sub>a node_assn\<^sup>k *\<^sub>a cap_assn\<^sup>k \<rightarrow>\<^sub>a x_assn"  
+    apply sepref_to_hoare unfolding x_assn_def x_add_impl_def x_add_def by (sep_auto simp: refine_pw_simps)
+
+  definition "l_assn \<equiv> is_nf (0::nat)"    
+  definition (in -) "l_init_impl N s cardV \<equiv> do {
+    l \<leftarrow> Array.new N (0::nat);
+    l \<leftarrow> Array.upd s cardV l;
+    return l
+  }"  
+  sepref_register l_init  
+  lemma [sepref_fr_rules]: "(l_init_impl N s, (PR_CONST l_init)) \<in> nat_assn\<^sup>k \<rightarrow>\<^sub>a l_assn"  
+    apply sepref_to_hoare unfolding l_assn_def l_init_def l_init_impl_def by sep_auto
+      
+  sepref_register l_get    
+  lemma [sepref_fr_rules]: "(uncurry Array.nth, uncurry (PR_CONST l_get)) \<in> l_assn\<^sup>k *\<^sub>a node_assn\<^sup>k \<rightarrow>\<^sub>a nat_assn"
+    apply sepref_to_hoare unfolding l_assn_def l_get_def by (sep_auto simp: refine_pw_simps)
+      
+  sepref_register l_set
+  lemma [sepref_fr_rules]: "(uncurry2 (\<lambda>a i x. Array.upd i x a), uncurry2 (PR_CONST l_set)) \<in> l_assn\<^sup>d *\<^sub>a node_assn\<^sup>k *\<^sub>a nat_assn\<^sup>k \<rightarrow>\<^sub>a l_assn"
+    apply sepref_to_hoare unfolding l_assn_def l_set_def by (sep_auto simp: refine_pw_simps split: prod.split)
+
+  abbreviation "xcf_assn \<equiv>  x_assn \<times>\<^sub>a cf_assn"    
+      
+  term pp_init_xcf2
+  sepref_register pp_init_xcf2    
+  sepref_thm pp_init_xcf_impl is "PR_CONST pp_init_xcf2" :: "am_assn\<^sup>k \<rightarrow>\<^sub>a xcf_assn"
+    unfolding pp_init_xcf2_def PR_CONST_def
+    by sepref  
+  concrete_definition (in -) pp_init_xcf_impl uses Network_Impl.pp_init_xcf_impl.refine_raw
+  lemmas [sepref_fr_rules] = pp_init_xcf_impl.refine[OF nwi_this]
+      
+  sepref_register push2  
+  sepref_thm push_impl is "uncurry2 (PR_CONST push2)" :: "x_assn\<^sup>d *\<^sub>a cf_assn\<^sup>d *\<^sub>a edge_assn\<^sup>k \<rightarrow>\<^sub>a xcf_assn"  
+    unfolding push2_def PR_CONST_def
+    by sepref
+  concrete_definition (in -) push_impl uses Network_Impl.push_impl.refine_raw is "(uncurry2 ?f,_)\<in>_"
+  lemmas [sepref_fr_rules] = push_impl.refine[OF nwi_this]
+    
+  sepref_register min_adj_label
+  sepref_thm min_adj_label_impl is "uncurry3 (PR_CONST min_adj_label)" :: "am_assn\<^sup>k *\<^sub>a cf_assn\<^sup>k *\<^sub>a l_assn\<^sup>k *\<^sub>a node_assn\<^sup>k \<rightarrow>\<^sub>a nat_assn"  
+    unfolding min_adj_label_def PR_CONST_def
+    by sepref  
+  concrete_definition (in -) min_adj_label_impl uses Network_Impl.min_adj_label_impl.refine_raw is "(uncurry3 ?f,_)\<in>_"
+  lemmas [sepref_fr_rules] = min_adj_label_impl.refine[OF nwi_this]    
+    
+  sepref_register relabel2
+  sepref_thm relabel_impl is "uncurry3 (PR_CONST relabel2)" :: "am_assn\<^sup>k *\<^sub>a cf_assn\<^sup>k *\<^sub>a l_assn\<^sup>d *\<^sub>a node_assn\<^sup>k \<rightarrow>\<^sub>a l_assn"  
+    unfolding relabel2_def PR_CONST_def
+    by sepref  
+  concrete_definition (in -) relabel_impl uses Network_Impl.relabel_impl.refine_raw is "(uncurry3 ?f,_)\<in>_"
+  lemmas [sepref_fr_rules] = relabel_impl.refine[OF nwi_this]    
+    
+  sepref_register discharge2
+  sepref_thm discharge_impl is "uncurry5 (PR_CONST discharge2)" 
+    :: "am_assn\<^sup>k *\<^sub>a x_assn\<^sup>d *\<^sub>a cf_assn\<^sup>d *\<^sub>a l_assn\<^sup>d *\<^sub>a n_assn\<^sup>d *\<^sub>a node_assn\<^sup>k \<rightarrow>\<^sub>a xcf_assn \<times>\<^sub>a l_assn \<times>\<^sub>a n_assn"  
+    unfolding discharge2_def PR_CONST_def
+    by sepref  
+  concrete_definition (in -) discharge_impl uses Network_Impl.discharge_impl.refine_raw is "(uncurry5 ?f,_)\<in>_"
+  lemmas [sepref_fr_rules] = discharge_impl.refine[OF nwi_this]    
   
-      
-      
+  sepref_register "init_CQ"
+    
+  sepref_thm init_CQ_impl is "uncurry (PR_CONST init_CQ)" 
+    :: "[\<lambda>(x,_). x=N]\<^sub>a nat_assn\<^sup>k *\<^sub>a am_assn\<^sup>k \<rightarrow> nat_assn \<times>\<^sub>a list_assn nat_assn"
+    unfolding init_CQ_def PR_CONST_def
+    apply (rewrite HOL_list.fold_custom_empty)
+    by sepref
+  concrete_definition (in -) init_CQ_impl uses Network_Impl.init_CQ_impl.refine_raw is "(uncurry ?f,_)\<in>_"
+  lemmas [sepref_fr_rules] = init_CQ_impl.refine[OF nwi_this]    
+    
+    
+  (* TODO: Move *)  
+  lemma (in -) rev_append_hnr[param,sepref_import_param]:
+    "(rev_append, rev_append) \<in> \<langle>A\<rangle>list_rel \<rightarrow> \<langle>A\<rangle>list_rel \<rightarrow> \<langle>A\<rangle>list_rel"
+    unfolding rev_append_def by parametricity
+    
+  sepref_register relabel_to_front2
+  sepref_thm relabel_to_front_impl is 
+    "uncurry (PR_CONST relabel_to_front2)" :: "[\<lambda>(x,_). x=N]\<^sub>a nat_assn\<^sup>k *\<^sub>a am_assn\<^sup>k \<rightarrow> cf_assn"  
+    unfolding relabel_to_front2_def PR_CONST_def
+    supply [[goals_limit = 1]]  
+    apply (rewrite in "Let [] _" HOL_list.fold_custom_empty)
+    apply (rewrite in "[_]" HOL_list.fold_custom_empty)
+    by sepref  
+  concrete_definition (in -) relabel_to_front_impl uses Network_Impl.relabel_to_front_impl.refine_raw is "(uncurry ?f,_)\<in>_"
+  lemmas [sepref_fr_rules] = relabel_to_front_impl.refine[OF nwi_this]
       
       
 end  
+  
+export_code relabel_to_front_impl in SML_imp module_name Relabel_To_Front
+  
+thm relabel_to_front_impl_def  
+  
+context Network_Impl begin
+  (*xxx, ctd here: Move this to Network locale! Define xxx_assn outside locales!?*)
+  
+  theorem relabel_to_front_impl_correct: 
+    assumes VN: "Graph.V c \<subseteq> {0..<N}"
+    assumes ABS_PS: "is_adj_map am"
+    shows "
+      <am_assn am ami> 
+        relabel_to_front_impl c s t N N ami
+      <\<lambda>cfi. \<exists>\<^sub>Acf. cf_assn cf cfi * \<up>(isMaxFlow (flow_of_cf cf))>\<^sub>t"
+  proof -
+    have AM: "(am, adjacent_nodes) \<in> nat_rel \<rightarrow> \<langle>nat_rel\<rangle>list_set_rel"
+      using ABS_PS
+      unfolding is_adj_map_def adjacent_nodes_def list_set_rel_def
+      by (auto simp: in_br_conv)
+        
+    note relabel_to_front2_refine[OF AM VN]    
+    also note relabel_to_front_correct
+    finally have R1: "relabel_to_front2 N am \<le> \<Down> (br flow_of_cf (RPreGraph c s t)) (SPEC isMaxFlow)" .  
 
-(*
-  Data structures:
-    flow, capacity: Matrix
+    have [simp]: "nofail (\<Down>R (RES X))" for R X by (auto simp: refine_pw_simps)
+        
+    note R2 = relabel_to_front_impl.refine[OF nwi_this, to_hnr, OF refl, unfolded autoref_tag_defs]
+    note R3 = hn_refine_ref[OF R1 R2, of ami N]  
+    note R4 = R3[unfolded hn_ctxt_def pure_def, THEN hn_refineD, simplified]
+      
+    show ?thesis  
+      by (sep_auto heap: R4 simp: pw_le_iff refine_pw_simps in_br_conv)
+  qed
+end    
 
-    neighbor list: Array: node \<rightarrow> node list
-    labeling: Array: node \<rightarrow> nat
-    excess: Array: node \<rightarrow> capacity
 
-    L_left, L_right: HOL list
-
-*)  
-  
-  
-  
-  
-  
-  
-  
-  
-  
-  
   
   
   
